state is func

Imp/State.lean
@@ -1,35 +1,13 @@
-inductive State
-  | init   : State
-  | update : State → String → Int → State
+import Mathlib.Logic.Function.Basic
 
-@[simp, reducible] def State.red (s: State) (x: String): Int :=
-  match s with
-  | State.init => 0 -- unbound variables are 0
-  | State.update s y m => bif x = y then m else s.red x
+def State := String → Int
+def State.nil: State := λ _ ↦ 0
 
-infix:110 "⇓" => State.red
+notation "⟪⟫" => State.nil
+notation s "⟪" x "≔" e "⟫" => Function.update s x e
 
-instance State.equiv: Setoid State where
-  r s₁ s₂ := ∀x, s₁⇓x = s₂⇓x
-  iseqv := {
-    refl := by simp
-    symm := by {
-      intro _ _ h _
-      apply Eq.symm
-      apply h
-    }
-    trans := by {
-      intro _ _ _ h₁ h₂ x
-      specialize h₁ x
-      specialize h₂ x
-      rw [h₁, h₂]
-    }
-  }
+#eval ⟪⟫ "x"
+#eval (⟪⟫⟪"x" ≔ 3⟫⟪"x" ≔ 4⟫) "x"
+#eval (⟪⟫⟪"x" ≔ 3⟫⟪"x" ≔ 4⟫⟪"x" ≔ 7⟫) "x"
 
-notation "⟦⟧" => State.init
-notation "⟦" x "↦" e "⟧" => State.update ⟦⟧ x e
-notation s "⟦" x "↦" e "⟧" => State.update s x e
-
-#check ⟦⟧
-#check ⟦"x"↦3⟧⟦"x"↦4⟧
-#eval  ⟦"x"↦3⟧⟦"x"↦4⟧⟦"x"↦7⟧⇓"x"
+theorem State.demo₁: (⟪⟫⟪"x"≔3⟫) = (⟪⟫⟪"x"≔4⟫⟪"x"≔3⟫) := by simp
