Imp/StackMachine/Structural.lean
@@ -1,0 +1,24 @@
+import Imp.StackMachine.Syntax
+import Mathlib.Data.List.Defs
+
+inductive Instr.Step: Instr × StackMachine → StackMachine → Prop where
+  | loadi₁:
+    Step (loadi n, ⟨pc, s, stk⟩) ⟨pc + 1, s, stk.concat n⟩
+
+  | load₁:
+    Step (load x, ⟨pc, s, stk⟩) ⟨pc + 1, s, stk.concat $ s x⟩
+
+  | add₁:
+    Step (add, ⟨pc, s, stk⟩) ⟨pc + 1, s, stk.concat (stk.take 2).sum⟩
+
+  | store₁:
+    Step (store x, ⟨pc, s, stk⟩) ⟨pc + 1, s⟪x ≔ stk.headD 0⟫, stk.tail⟩
+
+  | jmp₁:
+    Step (jmp n, ⟨pc, s, stk⟩) ⟨pc + 1 + n, s, stk⟩
+
+  | jmplt₁:
+    Step (jmplt n, ⟨pc, s, stk⟩) ⟨bif stk.tail.headD 0 < stk.headD 0 then pc + 1 + n else pc + 1, s, stk⟩
+
+  | jmpge₁:
+    Step (jmpge n, ⟨pc, s, stk⟩) ⟨bif stk.tail.headD 0 ≥ stk.headD 0 then pc + 1 + n else pc + 1, s, stk⟩
