Imp/StackMachine/Syntax.lean
@@ -1,0 +1,15 @@
+import Imp.State
+
+inductive Instr where
+  | loadi : Int → Instr
+  | load  : String → Instr
+  | add   : Instr
+  | store : String → Instr
+  | jmp   : Int → Instr
+  | jmplt : Int → Instr
+  | jmpge : Int → Instr
+
+structure StackMachine where
+  pc    : Int
+  state : State
+  stack : List Int
