Imp/Untyped/Equivalence.lean
@@ -1,18 +1,18 @@
-import Imp.Natural
-import Imp.Structural
-import Imp.Denot
+import Imp.Untyped.Natural
+import Imp.Untyped.Structural
+import Imp.Untyped.Denot
 
-theorem Com.Star.of_Nat {x: Com × State} (h: x ⟹ s): x ⇒* (skip, s) := by
+theorem Com.Star.of_Nat {x: Config} (h: x ⟹ s): x ⇒* (skip, s) := by
   induction h with
   | skip₁ => exact refl
   | ass₁ => exact single Step.ass₁
   | cat₁ _ _ _ ihc ihd => exact Star.cat ihc ihd
   | cond₁ hb _ ih => exact head Step.cond₁ (hb ▸ ih)
   | cond₂ hb _ ih => exact head Step.cond₁ (hb ▸ ih)
-  | wle₁ _ hb _ _ ihc ihw =>
-    exact head Step.wle₁ (head Step.cond₁ (hb ▸ Star.cat ihc ihw))
-  | wle₂ hb =>
-    exact head Step.wle₁ (head ((Step.cond_false hb).mpr rfl) refl)
+  | loop₁ _ hb _ _ ihc ihw =>
+    exact head Step.loop₁ (head Step.cond₁ (hb ▸ Star.cat ihc ihw))
+  | loop₂ hb =>
+    exact head Step.loop₁ (head ((Step.cond_false hb).mpr rfl) refl)
 
 lemma Com.Nat.of_Step (h₁: x ⇒ y) (h₂: y ⟹ s): x ⟹ s := by
   induction h₁ generalizing s with
@@ -22,16 +22,16 @@ lemma Com.Nat.of_Step (h₁: x ⇒ y) (h₂: y ⟹ s): x ⟹ s := by
     cases h₂ with
     | cat₁ w hc hd => exact cat₁ w (ih hc) hd
   | cond₁ => exact cond_ext''.mpr h₂
-  | wle₁ => rw [wle_unfold]; exact h₂
+  | loop₁ => rw [loop_unfold]; exact h₂
 
 theorem Com.Nat.of_Star (h: x ⇒* (skip, t)): x ⟹ t := by
   induction h using Star.head_induction_on with
   | refl => exact skip₁
   | head x x' ht => cases x' <;> exact of_Step x ht
 
-theorem Com.Star_iff_Nat: x ⇒* (skip, t) ↔ x ⟹ t := ⟨Nat.of_Star, Star.of_Nat⟩
+theorem Com.Star_iff_Nat: x ⇒* (skip, t) = x ⟹ t := propext ⟨Nat.of_Star, Star.of_Nat⟩
 
-theorem Com.denot.of_Nat {x: Com × State} (h: x ⟹ t): (x.2, t) ∈ ⟦x.1⟧ := by
+theorem Com.denot.of_Nat {x: Config} (h: x ⟹ t): (x.2, t) ∈ ⟦x.1⟧ := by
   induction h with
   | skip₁ => rfl
   | ass₁  => rfl
@@ -43,12 +43,12 @@ theorem Com.denot.of_Nat {x: Com × State} (h: x ⟹ t): (x.2, t) ∈ ⟦x.1⟧ 
   | cond₂ hb _ ih =>
     simp [denot]
     exact Or.inr ⟨ih, hb⟩
-  | wle₁ t hb _ _ ih₁ ih₂ =>
-    rw [wle_unfold]
+  | loop₁ t hb _ _ ih₁ ih₂ =>
+    rw [loop_unfold]
     simp [denot]
     exact Or.inl ⟨⟨t, ⟨ih₁, ih₂⟩⟩, hb⟩
-  | wle₂ hb =>
-    rw [wle_unfold]
+  | loop₂ hb =>
+    rw [loop_unfold]
     simp [denot]
     exact Or.inr hb
 
@@ -70,8 +70,8 @@ theorem Com.Nat.of_denot (h: (s, t) ∈ ⟦c⟧): (c, s) ⟹ t := by
     | inr h =>
       cases h with | intro h hb =>
         exact cond₂ hb (ih₂ h)
-  | wle b c ih =>
-    suffices ⟦wle b c⟧ ⊆ {s | (wle b c, s.1) ⟹ s.2} by apply this
+  | loop b c ih =>
+    suffices ⟦loop b c⟧ ⊆ {s | (loop b c, s.1) ⟹ s.2} by apply this
     apply OrderHom.lfp_le
     intro ss h
     cases ss with | mk =>
@@ -79,10 +79,10 @@ theorem Com.Nat.of_denot (h: (s, t) ∈ ⟦c⟧): (c, s) ⟹ t := by
       | inl h =>
         cases h with | intro h hb =>
           cases h with | intro w h =>
-            exact wle₁ w hb (ih h.left) h.right
+            exact loop₁ w hb (ih h.left) h.right
       | inr h =>
         cases h with | intro hq hb =>
           simp at hq
-          exact hq ▸ wle₂ hb
+          exact hq ▸ loop₂ hb
 
-theorem Com.Nat_iff_denot: (s, t) ∈ ⟦c⟧ ↔ (c, s) ⟹ t := ⟨Nat.of_denot, denot.of_Nat⟩
+theorem Com.Nat_iff_denot: ((s, t) ∈ ⟦c⟧) = (c, s) ⟹ t := propext ⟨Nat.of_denot, denot.of_Nat⟩
